StandardLibrary/src/StandardLibrary.dfy
@@ -184,8 +184,8 @@ module StandardLibrary {
     if a < b then a else b
   }
 
-  function method Fill<T>(value: T, n: nat): seq<T>
-    ensures |Fill(value, n)| == n
+  function method Fill<T>(value: T, n: uint64): seq<T>
+    ensures |Fill(value, n)| == n as nat
     ensures forall i :: 0 <= i < n ==> Fill(value, n)[i] == value
   {
     seq(n, _ => value)
