AwsCryptographicMaterialProviders/dafny/AwsCryptographicMaterialProviders/src/Keyrings/RawECDHKeyring.dfy
@@ -16,6 +16,7 @@ include "./AwsKms/Constants.dfy"
 module {:options "/functionSyntax:4" } RawECDHKeyring {
   import opened StandardLibrary
   import opened UInt = StandardLibrary.UInt
+  import opened StandardLibrary.MemoryMath
   import opened String = StandardLibrary.String
   import opened Actions
   import opened Wrappers
@@ -40,23 +41,29 @@ module {:options "/functionSyntax:4" } RawECDHKeyring {
 
   predicate ValidPublicKeyLength(p: seq<uint8>)
   {
-    && (|p| == ECDH_PUBLIC_KEY_LEN_ECC_NIST_256 ||
-        |p| == ECDH_PUBLIC_KEY_LEN_ECC_NIST_384 ||
-        |p| == ECDH_PUBLIC_KEY_LEN_ECC_NIST_521)
+    SequenceIsSafeBecauseItIsInMemory(p);
+    var len := |p| as uint64;
+    && (len == ECDH_PUBLIC_KEY_LEN_ECC_NIST_256 ||
+        len == ECDH_PUBLIC_KEY_LEN_ECC_NIST_384 ||
+        len == ECDH_PUBLIC_KEY_LEN_ECC_NIST_521)
   }
 
   predicate ValidCompressedPublicKeyLength(p: seq<uint8>)
   {
-    && (|p| == ECDH_PUBLIC_KEY_COMPRESSED_LEN_ECC_NIST_256 ||
-        |p| == ECDH_PUBLIC_KEY_COMPRESSED_LEN_ECC_NIST_384 ||
-        |p| == ECDH_PUBLIC_KEY_COMPRESSED_LEN_ECC_NIST_521)
+    SequenceIsSafeBecauseItIsInMemory(p);
+    var len := |p| as uint64;
+    && (len == ECDH_PUBLIC_KEY_COMPRESSED_LEN_ECC_NIST_256 ||
+        len == ECDH_PUBLIC_KEY_COMPRESSED_LEN_ECC_NIST_384 ||
+        len == ECDH_PUBLIC_KEY_COMPRESSED_LEN_ECC_NIST_521)
   }
 
   predicate ValidProviderInfoLength(p: seq<uint8>)
   {
-    (|p| == ECDH_PROVIDER_INFO_256_LEN as int ||
-     |p| == ECDH_PROVIDER_INFO_384_LEN as int ||
-     |p| == ECDH_PROVIDER_INFO_521_LEN as int
+    SequenceIsSafeBecauseItIsInMemory(p);
+    var len := |p| as uint64;
+    (len == ECDH_PROVIDER_INFO_256_LEN as uint64 ||
+     len == ECDH_PROVIDER_INFO_384_LEN as uint64 ||
+     len == ECDH_PROVIDER_INFO_521_LEN as uint64
     )
   }
 
@@ -369,7 +376,8 @@ module {:options "/functionSyntax:4" } RawECDHKeyring {
       //# For the encrypted data key to match:
       var edksToAttempt :- FilterWithResult(filter, input.encryptedDataKeys);
 
-      if (0 == |edksToAttempt|) {
+      SequenceIsSafeBecauseItIsInMemory(edksToAttempt);
+      if (0 == |edksToAttempt| as uint64) {
         var errorMessage :- ErrorMessages.IncorrectDataKeys(input.encryptedDataKeys, input.materials.algorithmSuite);
         return Failure(E(errorMessage));
       }
@@ -462,13 +470,14 @@ module {:options "/functionSyntax:4" } RawECDHKeyring {
         return Success(false);
       }
 
+      SequenceIsSafeBecauseItIsInMemory(providerInfo);
       :- Need(
-        && |providerInfo| <= ECDH_PROVIDER_INFO_521_LEN as int
+        && |providerInfo| as uint64 <= ECDH_PROVIDER_INFO_521_LEN as uint64
         && ValidProviderInfoLength(providerInfo),
         E("EDK ProviderInfo longer than expected")
       );
 
-      var keyringVersion := providerInfo[0];
+      var keyringVersion := providerInfo[0 as uint32];
       :- Need(
         //= aws-encryption-sdk-specification/framework/raw-ecdh-keyring.md#ondecrypt
         //# - The deserialized version value in the [key provider information](#key-provider-information) MUST match `0x01`.
@@ -476,11 +485,11 @@ module {:options "/functionSyntax:4" } RawECDHKeyring {
         E("Incorrect Keyring version found in provider info.")
       );
 
-      var recipientPublicKeyLength := SeqToUInt32(providerInfo[ECDH_PROVIDER_INFO_RPL_INDEX..ECDH_PROVIDER_INFO_RPK_INDEX]) as int;
-      var recipientPublicKeyLengthIndex := ECDH_PROVIDER_INFO_RPK_INDEX as int + recipientPublicKeyLength;
-      var senderPublicKeyIndex := recipientPublicKeyLengthIndex + ECDH_PROVIDER_INFO_PUBLIC_KEY_LEN as int;
+      var recipientPublicKeyLength := SeqToUInt32(providerInfo[ECDH_PROVIDER_INFO_RPL_INDEX..ECDH_PROVIDER_INFO_RPK_INDEX]);
+      var recipientPublicKeyLengthIndex := ECDH_PROVIDER_INFO_RPK_INDEX as uint64 + recipientPublicKeyLength as uint64;
+      var senderPublicKeyIndex := recipientPublicKeyLengthIndex + ECDH_PROVIDER_INFO_PUBLIC_KEY_LEN;
       :- Need(
-        recipientPublicKeyLengthIndex + 4 < |providerInfo|,
+        recipientPublicKeyLengthIndex + 4 < |providerInfo| as uint64,
         E("Key Provider Info Serialization Error. Serialized length less than expected.")
       );
       var providerInfoRecipientPublicKey := providerInfo[ECDH_PROVIDER_INFO_RPK_INDEX..recipientPublicKeyLengthIndex];
@@ -597,13 +606,14 @@ module {:options "/functionSyntax:4" } RawECDHKeyring {
 
       var providerWrappedMaterial :- EdkWrapping.GetProviderWrappedMaterial(ciphertext, suite);
 
+      SequenceIsSafeBecauseItIsInMemory(providerInfo);
       :- Need(
-        && |providerInfo| <= ECDH_PROVIDER_INFO_521_LEN as int
+        && |providerInfo| as uint64 <= ECDH_PROVIDER_INFO_521_LEN as uint64
         && ValidProviderInfoLength(providerInfo),
         E("EDK ProviderInfo longer than expected")
       );
 
-      var keyringVersion := providerInfo[0];
+      var keyringVersion := providerInfo[0 as uint32];
       :- Need(
         [keyringVersion] == RAW_ECDH_KEYRING_VERSION,
         E("Incorrect Keyring version found in provider info.")
@@ -611,11 +621,11 @@ module {:options "/functionSyntax:4" } RawECDHKeyring {
 
       //= aws-encryption-sdk-specification/framework/raw-ecdh-keyring.md#ondecrypt
       //# - The [ciphertext](#ciphertext) and [key provider information](#key-provider-information) MUST be successfully deserialized.
-      var recipientPublicKeyLength := SeqToUInt32(providerInfo[ECDH_PROVIDER_INFO_RPL_INDEX..ECDH_PROVIDER_INFO_RPK_INDEX]) as int;
-      var recipientPublicKeyLengthIndex := ECDH_PROVIDER_INFO_RPK_INDEX as int + recipientPublicKeyLength;
-      var senderPublicKeyIndex := recipientPublicKeyLengthIndex + ECDH_PROVIDER_INFO_PUBLIC_KEY_LEN as int;
+      var recipientPublicKeyLength := SeqToUInt32(providerInfo[ECDH_PROVIDER_INFO_RPL_INDEX..ECDH_PROVIDER_INFO_RPK_INDEX]);
+      var recipientPublicKeyLengthIndex := ECDH_PROVIDER_INFO_RPK_INDEX as uint64 + recipientPublicKeyLength as uint64;
+      var senderPublicKeyIndex := recipientPublicKeyLengthIndex + ECDH_PROVIDER_INFO_PUBLIC_KEY_LEN;
       :- Need(
-        recipientPublicKeyLengthIndex + 4 < |providerInfo|,
+        recipientPublicKeyLengthIndex + 4 < |providerInfo| as uint64,
         E("Key Provider Info Serialization Error. Serialized length less than expected.")
       );
       var providerInfoRecipientPublicKey := providerInfo[ECDH_PROVIDER_INFO_RPK_INDEX..recipientPublicKeyLengthIndex];
@@ -765,10 +775,10 @@ module {:options "/functionSyntax:4" } RawECDHKeyring {
       )
     );
 
-    var compresedPublicKey :- maybeCompressedPublicKey
+    var compressedPublicKey :- maybeCompressedPublicKey
     .MapFailure(e => Types.AwsCryptographyPrimitives( AwsCryptographyPrimitives := e));
 
-    return Success(compresedPublicKey.compressedPublicKey);
+    return Success(compressedPublicKey.compressedPublicKey);
   }
 
   method {:vcs_split_on_every_assert} DecompressPublicKey(
