AwsCryptographyPrimitives/src/Signature.dfy
@@ -7,6 +7,7 @@ module {:extern "Signature"} Signature {
 
   import opened Wrappers
   import opened UInt = StandardLibrary.UInt
+  import opened StandardLibrary.MemoryMath
   import Types = AwsCryptographyPrimitivesTypes
 
   datatype SignatureKeyPair = SignatureKeyPair(verificationKey: seq<uint8>, signingKey: seq<uint8>)
@@ -19,7 +20,7 @@ module {:extern "Signature"} Signature {
     case ECDSA_P384 => 103
   }
 
-  function method FieldSize(signatureAlgorithm: Types.ECDSASignatureAlgorithm): nat {
+  function method FieldSize(signatureAlgorithm: Types.ECDSASignatureAlgorithm): uint64 {
     match signatureAlgorithm
     case ECDSA_P256 => assert 1 + (256 + 7) / 8 == 33; 33
     case ECDSA_P384 => assert 1 + (384 + 7) / 8 == 49; 49
@@ -37,13 +38,14 @@ module {:extern "Signature"} Signature {
               //# The signing key MUST fit the specification described by the signature
               //# algorithm (algorithm-suites.md#signature-algorithm) included in this
               //# encryption material's algorithm suite (Section 2.3.3.2.1).
-              && |sigKeyPair.verificationKey| == FieldSize(input.signatureAlgorithm)
+              && |sigKeyPair.verificationKey| == FieldSize(input.signatureAlgorithm) as nat
             // && IsValidSignatureKeyPair(sigKeyPair)
             case Failure(_) => true
   {
     var sigKeyPair :- ExternKeyGen(input.signatureAlgorithm);
+    SequenceIsSafeBecauseItIsInMemory(sigKeyPair.verificationKey);
 
-    :- Need(|sigKeyPair.verificationKey| == FieldSize(input.signatureAlgorithm),
+    :- Need(|sigKeyPair.verificationKey| as uint64 == FieldSize(input.signatureAlgorithm) as uint64,
             Types.AwsCryptographicPrimitivesError(
               message := "Incorrect verification-key length from ExternKeyGen."
             ));
@@ -58,14 +60,14 @@ module {:extern "Signature"} Signature {
   // Generate an ECDSA key pair
   // Verification key, a.k.a public key, is in X9.62 compressed format
   // Signing Key, a.k.a private key, is in DER-encoded
-  method {:extern "Signature.ECDSA", "ExternKeyGen"} ExternKeyGen(
+  method {:extern "Signature.ECDSA", "ExternKeyGen"} {:axiom} ExternKeyGen(
     s: Types.ECDSASignatureAlgorithm
   ) returns (res: Result<SignatureKeyPair, Types.Error>)
     ensures res.Success? ==> IsValidSignatureKeyPair(res.value)
 
   // sign the message with the private key
   // private signing key is DER-encoded
-  method {:extern "Signature.ECDSA", "Sign"} Sign(
+  method {:extern "Signature.ECDSA", "Sign"} {:axiom} Sign(
     s: Types.ECDSASignatureAlgorithm,
     key: seq<uint8>,
     msg: seq<uint8>
