StandardLibrary/src/Actions.dfy
@@ -1,7 +1,6 @@
 // Copyright Amazon.com Inc. or its affiliates. All Rights Reserved.
 // SPDX-License-Identifier: Apache-2.0
 
-include "../../libraries/src/Wrappers.dfy"
 include "../../libraries/src/Collections/Sequences/Seq.dfy"
 include "MemoryMath.dfy"
 
