StandardLibrary/src/MemoryMath.dfy
@@ -6,10 +6,12 @@
 // To convince Dafny that this is true, we have the following functions
 // with assumptions as needed.
 
+include "../../libraries/src/Wrappers.dfy"
 include "UInt.dfy"
 
 module {:options "--function-syntax:4"} StandardLibrary.MemoryMath {
   import opened UInt
+  import opened Wrappers
 
   // This is safe because it is being held in memory
   lemma {:axiom} ValueIsSafeBecauseItIsInMemory(value : nat)
@@ -21,10 +23,32 @@ module {:options "--function-syntax:4"} StandardLibrary.MemoryMath {
     ValueIsSafeBecauseItIsInMemory(|value|);
   }
 
+  lemma SetIsSafeBecauseItIsInMemory<T>(value : set<T>)
+    ensures HasUint64Size(|value|)
+  {
+    ValueIsSafeBecauseItIsInMemory(|value|);
+  }
+
+  lemma OptionalSequenceIsSafeBecauseItIsInMemory<T>(value : Option<seq<T>>)
+    ensures value.Some? ==> HasUint64Len(value.value)
+  {
+    if value.Some? {
+      SequenceIsSafeBecauseItIsInMemory(value.value);
+    }
+  }
+
   lemma MapIsSafeBecauseItIsInMemory<K, V>(value : map<K, V>)
     ensures HasUint64Size(|value|)
   {
     ValueIsSafeBecauseItIsInMemory(|value|);
+  }
+
+  lemma OptionalMapIsSafeBecauseItIsInMemory<K, V>(value : Option<map<K, V>>)
+    ensures value.Some? ==> HasUint64Size(|value.value|)
+  {
+    if value.Some? {
+      ValueIsSafeBecauseItIsInMemory(|value.value|);
+    }
   }
 
   lemma ArrayIsSafeBecauseItIsInMemory<T>(value : array<T>)
